\section*{Problema 07}

\textbf{Show that}

\begin{equation*}
    f(x) = log\left ( \sum_{i=1}^n exp(x_i) \right )
\end{equation*}

\textbf{is convex}


Comprobando que $f(\alpha x_1 + (1-\alpha)x_2) \leq \alpha f(x_1) + (1-\alpha)f(x_2)$, se obtiene lo siguiente:

\begin{align*}
    f(\alpha x_1 + (1-\alpha)x_2) & = log \left ( \sum exp((\alpha x_1 + (1-\alpha)x_2)) \right )                                 \\
                                  & = log \left (\sum exp(\alpha x_1) exp((1-\alpha)x_2) \right )                                 \\
                                  & = log \left (\sum exp(x_1)^\alpha exp(x_2)^(1-\alpha) \right )                                \\
                                  & \leq \left (\sum exp(x_1)^\alpha \sum  exp(x_2)^(1-\alpha)  \right )                          \\
                                  & \leq \alpha log \left ( \sum exp(x_1) \right ) + (1-\alpha) log \left (\sum exp(x_2) \right ) \\
    f(\alpha x_1 + (1-\alpha)x_2) & \leq \alpha f(x_1) + (1-\alpha) f(x_2)
\end{align*}

por lo tanto, $f$ es convexa.